hinata_mikami/gc/output/gc/proofs/proof_Heap_sweep.v
@@ -13,72 +13,52 @@ Proof.
   Heap_sweep_prelude.
 
   rep <-! liRStep; liShow.
-  (* Goal 1 *)
+
   {
     iRename select
-    ([∗ list] k ↦ x ∈ (id <$> h),
-      ∃ (l0 n : loc) (m : bool), _)%I
-    into "Hnodes".
+      ([∗ list] i ↦ v ∈ vals,
+        ∃ (l n : loc) (m : bool), _)%I
+      into "Hnodes".
 
-    assert (Hmap_vals : (id <$> h) = h).
+    set (idx := Z.to_nat (ic - 1)).
+
+    assert (Hidx_locs : (idx < length locs)%nat).
     {
-      autorewrite with lithium_rewrite.
-      done.
+      unfold idx.
+      lia.
     }
 
-    assert (Hmap_locs : (id <$> h0) = h0).
+    assert (Hidx_vals : (idx < length vals)%nat).
     {
-      autorewrite with lithium_rewrite.
-      done.
+      rewrite <- H9.
+      exact Hidx_locs.
     }
-
-    assert (Hmap_nexts : (id <$> h1) = h1).
-    {
-      autorewrite with lithium_rewrite.
-      done.
-    }
-
-    assert (Hmap_marks : (id <$> h2) = h2).
-    {
-      autorewrite with lithium_rewrite.
-      done.
-    }
-
-    iEval (
-      rewrite Hmap_vals
-              Hmap_locs
-              Hmap_nexts
-              Hmap_marks
-    ) in "Hnodes".
-
-
-    assert (H0_vals : (0 < length h)%nat) by lia.
 
     destruct
-      (lookup_lt_is_Some_2 h 0%nat H0_vals)
-      as [vi Hvi].
+    (lookup_lt_is_Some_2 vals idx Hidx_vals)
+    as [vi Hvi].
 
     iDestruct
       (big_sepL_lookup_acc_impl
-        0%nat vi Hvi
+        idx vi Hvi
         with "Hnodes")
       as "(HiNode & Hclose)".
 
     iDestruct "HiNode" as
-      (node_l next0 mark0)
-      "(%Hloc0 & %Hnext0 & %Hmark0 &
+      (node_l next_i mark_i)
+      "(%Hloc_i & %Hnext_i & %Hmark_i &
         Hguard & Hfree)".
 
     assert (Hloc_total :
-      h0 !! 0%nat = Some (h0 !!! 0%nat)).
+      locs !! idx = Some (locs !!! idx)).
     {
       apply list_lookup_lookup_total_lt.
-      lia.
+      exact Hidx_locs.
     }
 
-    assert (node_l = h0 !!! 0%nat) as Heq_node.
+    assert (node_l = locs !!! idx) as Heq_node.
     {
-      rewrite Hloc0 in Hloc_total.
+      rewrite Hloc_i in Hloc_total.
       injection Hloc_total as Heq_node.
       exact Heq_node.
     }
@@ -90,7 +70,113 @@ Proof.
     rep <-! liRStep; liShow.
 
     - iRename select
-      ((h0 !!! Z.to_nat 0) ◁ₗ[_, Owned] _ @ _)%I
+      ((locs !!! idx) ◁ₗ[_, Owned] _ @ _)%I
+      into "Hnode".
+
+      set (P := fun (k : nat) (y : Z) =>
+        (∃ (l0 n : loc) (m : bool),
+          ⌜locs !! k = Some l0⌝ ∗
+          ⌜nexts !! k = Some n⌝ ∗
+          ⌜marks !! k = Some m⌝ ∗
+          guarded true
+            (l0 ◁ₗ[π, Owned]
+              # -[# y; # n; # m]
+              @ (◁ (Node_ty <INST!>))) ∗
+          freeable_nz l0
+            (ly_size (use_layout_alg' Node_sls))
+            1 HeapAlloc)%I).
+
+      iSpecialize ("Hclose" $! P).
+
+      iSpecialize ("Hclose" with "[]").
+      {
+        iModIntro.
+        iIntros (k y) "%Hlookup %Hneq HP".
+        unfold P.
+        iExact "HP".
+      }
+
+      iAcquireCredits as "Hcred".
+
+      iRevert "Hnode Hfree Hclose".
+
+      rep liRStep; liShow.
+
+      iRename select
+        (P idx vi -∗ [∗ list] k ↦ y ∈ vals, P k y)%I
+        into "Hclose".
+
+      iRename select
+        ((locs !!! idx) ◁ₗ[_, Owned] _ @ _)%I
+        into "Hnode".
+
+      iRename select
+        (freeable_nz (locs !!! idx) _ 1 HeapAlloc)%I
+        into "Hfree".
+
+      iApply
+      (prove_with_subtype_big_sepL_acc
+        _ _ _ _ vals P idx vi _
+        with "Hclose").
+
+      unfold P.
+      rep liRStep; liShow.
+
+      iApply prove_with_subtype_default.
+
+
+(* 
+    set (idx := Z.to_nat (length locs - 1)).
+
+    assert (Hidx_locs : (idx < length locs)%nat).
+    {
+      unfold idx.
+      lia.
+    }
+
+    assert (Hidx_vals : (idx < length vals)%nat).
+    {
+      rewrite <- H9.
+      exact Hidx_locs.
+    }
+
+    destruct
+    (lookup_lt_is_Some_2 vals idx Hidx_vals)
+    as [vi Hvi].
+
+    iDestruct
+    (big_sepL_lookup_acc_impl
+      idx vi Hvi
+      with "Hnodes")
+    as "(HiNode & Hclose)".
+
+    iDestruct "HiNode" as
+    (node_l next_i mark_i)
+    "(%Hloc_i & %Hnext_i & %Hmark_i &
+      Hguard & Hfree)".
+
+    assert (Hloc_total :
+      locs !! idx = Some (locs !!! idx)).
+    {
+      apply list_lookup_lookup_total_lt.
+      exact Hidx_locs.
+    }
+
+    assert (node_l = locs !!! idx) as Heq_node.
+    {
+      rewrite Hloc_i in Hloc_total.
+      injection Hloc_total as Heq_node.
+      exact Heq_node.
+    }
+
+    subst node_l.
+
+    apply_update updateable_strip_guards.
+
+    rep <-! liRStep; liShow.
+
+    - iRename select
+      ((locs !!! idx) ◁ₗ[_, Owned] _ @ _)%I
       into "Hnode".
 
       iAcquireCredits as "Hcred".
@@ -102,13 +188,11 @@ Proof.
       rep liRStep; liShow.
 
       iRename select
-      ((h0 !!! Z.to_nat 0) ◁ₗ[π, Owned] _ @ _)%I
-      into "Hnode".
+        ((locs !!! idx) ◁ₗ[_, Owned] _ @ _)%I
+        into "Hnode".
 
       iRename select
-        (freeable_nz (h0 !!! 0%nat)
-          (ly_size (use_layout_alg' Node_sls))
-          1 HeapAlloc)%I
+        (freeable_nz (locs !!! idx) _ 1 HeapAlloc)%I
         into "Hfree".
 
       iRename select
@@ -117,9 +201,9 @@ Proof.
 
       set (P := fun (k : nat) (y : Z) =>
       (∃ (l0 n : loc) (m : bool),
-        ⌜h0 !! k = Some l0⌝ ∗
-        ⌜h1 !! k = Some n⌝ ∗
-        ⌜h2 !! k = Some m⌝ ∗
+        ⌜locs !! k = Some l0⌝ ∗
+        ⌜nexts !! k = Some n⌝ ∗
+        ⌜marks !! k = Some m⌝ ∗
         guarded true
           (l0 ◁ₗ[π, Owned]
             # -[# y; # n; # m]
@@ -127,7 +211,7 @@ Proof.
         freeable_nz l0
           (ly_size (use_layout_alg' Node_sls))
           1 HeapAlloc)%I).
-      
+
       iSpecialize ("Hclose" $! P).
 
       iSpecialize ("Hclose" with "[]").
@@ -138,28 +222,21 @@ Proof.
         iExact "HP".
       }
 
-      iRevert "Hnode Hfree Hclose".
-      iIntros "Hnode Hfree Hclose".
-
-      rep liRStep; liShow.
-
       iApply
-        (prove_with_subtype_big_sepL_acc
-          _ _ _ _ h P 0%nat vi _
-          with "Hclose").
+      (prove_with_subtype_big_sepL_acc
+        _ _ _ _ vals P idx vi _
+        with "Hclose").
 
       unfold P.
 
-      rep liRStep; liShow.
-      
+      rep liRStep; liShow. *)
 
     
-
   }
-  (* Goal 2 *)
   {
 
   }
+
 
   all: print_remaining_goal.
   Unshelve. all: sidecond_solver.
